projects/task3/VC/thm_apply_proof_manual__.v
@@ -1,0 +1,330 @@
+Require Import Coq.ZArith.ZArith.
+Require Import Coq.Bool.Bool.
+Require Import Coq.Strings.String.
+Require Import Coq.Lists.List.
+Require Import Coq.Classes.RelationClasses.
+Require Import Coq.Classes.Morphisms.
+Require Import Coq.micromega.Psatz.
+Require Import Coq.Sorting.Permutation.
+From AUXLib Require Import int_auto Axioms Feq Idents List_lemma VMap.
+Require Import SetsClass.SetsClass. Import SetsNotation.
+From SimpleC.SL Require Import Mem SeparationLogic.
+Require Import thm_apply_goal.
+Require Import Logic.LogicGenerator.demo932.Interface.
+Local Open Scope Z_scope.
+Local Open Scope sets.
+Local Open Scope string.
+Local Open Scope list.
+Import naive_C_Rules.
+From SimpleC.EE Require Import ast_lib.
+From SimpleC.EE Require Import malloc.
+From SimpleC.EE Require Import super_poly_sll2.
+Local Open Scope sac.
+
+Lemma sll_zero_right : forall (A : Type) P (storeA: addr -> A -> Assertion) s1 s2 l Q,
+  l <> nil ->
+  P ** sll storeA s1 s2 0 l |-- Q.
+Proof.
+  intros.
+  unfold sll.
+  destruct l.
+  - contradiction.
+  - unfold NULL.
+    Intros y.
+    contradiction.
+Qed.
+
+Lemma proof_of_sub_thm_return_wit_1 : sub_thm_return_wit_1.
+Proof.
+  pre_process.
+  rewrite H.
+  unfold sll_var_sub_list.
+  pose proof (sll_zero store_var_sub_cell "var_sub_list"
+  "next" 0 l).
+  unfold NULL in H0.
+  assert (0 = 0).
+  lia.
+  pose proof (H0 H1); clear H0 H1.
+  destruct l.
+  unfold thm_subst.
+  entailer!.
+  apply sll_zero_right.
+  discriminate.
+Qed.
+
+Lemma proof_of_sub_thm_return_wit_2 : sub_thm_return_wit_2.
+Proof.
+  pre_process.
+  rewrite H4.
+  rewrite H1.
+  rewrite H0.
+  unfold sll_var_sub_list.
+  unfold sll.
+  fold (sll store_var_sub_cell "var_sub_list" "next").
+  Exists lis_next.
+  unfold thm_subst.
+  fold thm_subst.
+  entailer!.
+  destruct qt.
+  - admit.
+  - unfold store_term_res at 2. admit.
+Admitted.
+
+Lemma proof_of_sub_thm_return_wit_3 : sub_thm_return_wit_3.
+Proof.
+  pre_process.
+  unfold store_term_res.
+  (* unfold sll_var_sub_list at 2. unfold sll.
+  destruct (thm_subst t l) eqn:E.
+  unfold store_term. *)
+Admitted.
+
+Lemma proof_of_sub_thm_partial_solve_wit_3_pure : sub_thm_partial_solve_wit_3_pure.
+Proof.
+  pre_process.
+  sep_apply store_term_unfold.
+  sep_apply store_term_unfold.
+  unfold store_string, NULL.
+  Intros n1 n2.
+  entailer!.
+Qed.
+
+Lemma proof_of_sub_thm_which_implies_wit_1 : sub_thm_which_implies_wit_1.
+Proof.
+  pre_process.
+  destruct l.
+  - unfold sll_var_sub_list.
+    unfold sll.
+    Intros.
+    unfold NULL in H0.
+    lia.
+  - simpl.
+    Intros x.
+    unfold store_var_sub_cell.
+    Intros y.
+    Exists x y v l.
+    sep_apply store_term_unfold.
+    entailer!.
+Qed.
+
+Lemma proof_of_sub_thm_which_implies_wit_2 : sub_thm_which_implies_wit_2.
+Proof.
+  pre_process.
+Admitted.
+
+Lemma proof_of_separate_imply_return_wit_1 : separate_imply_return_wit_1.
+Proof.
+  pre_process.
+  unfold store_imply_res.
+  unfold sep_impl.
+  destruct trm; unfold termtypeID, NULL in *.
+  - entailer!.
+  - entailer!.
+  - contradiction.
+  - entailer!.
+Qed.
+
+Lemma proof_of_separate_imply_return_wit_2 : separate_imply_return_wit_2.
+Proof.
+  pre_process.
+  unfold store_imply_res.
+  unfold sep_impl.
+  rewrite H1.
+  destruct lt; try lia.
+  - entailer!.
+  - entailer!.
+  - contradiction.
+  - entailer!.
+Qed.
+
+Lemma proof_of_separate_imply_return_wit_3 : separate_imply_return_wit_3.
+Proof.
+  pre_process.
+  unfold store_imply_res.
+  unfold sep_impl.
+  rewrite H4.
+  rewrite H1.
+  destruct ll.
+  - entailer!.
+  - entailer!.
+  - entailer!.
+  - entailer!.
+Qed.
+
+Lemma proof_of_separate_imply_return_wit_4 : separate_imply_return_wit_4.
+Proof.
+  pre_process.
+  unfold store_imply_res.
+  unfold sep_impl.
+  rewrite H6.
+  rewrite H3.
+  rewrite H0.
+  destruct llctype.
+  - entailer!.
+  - entailer!.
+  - entailer!.
+  - entailer!.
+  - entailer!.
+  - entailer!.
+  - entailer!.
+  - contradiction.
+Qed. 
+
+Lemma proof_of_separate_imply_return_wit_5 : separate_imply_return_wit_5.
+Proof.
+  pre_process.
+  unfold store_imply_res.
+  unfold sep_impl.
+  rewrite H6.
+  rewrite H3.
+  rewrite H0.
+  destruct llctype.
+  - unfold ctID in H; lia.
+  - unfold ctID in H; lia.
+  - unfold ctID in H; lia.
+  - unfold ctID in H; lia.
+  - unfold ctID in H; lia.
+  - unfold ctID in H; lia.
+  - unfold ctID in H; lia.
+  - Exists t1' t2'.
+  entailer!.
+    unfold store_ImplyProp at 2.
+    admit.
+Admitted.
+
+Lemma proof_of_separate_imply_which_implies_wit_1 : separate_imply_which_implies_wit_1.
+Proof.
+  pre_process.
+  sep_apply store_term_unfold.
+  unfold NULL.
+  entailer!.
+Qed.
+
+Lemma proof_of_separate_imply_which_implies_wit_2 : separate_imply_which_implies_wit_2.
+Proof.
+  pre_process.
+  sep_apply store_term'_Apply; unfold NULL in *.
+  Intros lt rt y z.
+  Exists z y lt rt.
+  rewrite H3.
+  entailer!.
+  lia.
+  lia.
+Qed.
+
+Lemma proof_of_separate_imply_which_implies_wit_3 : separate_imply_which_implies_wit_3.
+Proof.
+  pre_process.
+  sep_apply store_term_unfold.
+  unfold NULL.
+  entailer!.
+Qed.
+
+
+Lemma proof_of_separate_imply_which_implies_wit_4 : separate_imply_which_implies_wit_4.
+Proof.
+  pre_process.
+  sep_apply store_term'_Apply; unfold NULL in *.
+  Intros ll lr y z.
+  Exists z y ll lr.
+  entailer!.
+  lia.
+  lia.
+Qed. 
+
+Lemma proof_of_separate_imply_which_implies_wit_5 : separate_imply_which_implies_wit_5.
+Proof.
+  pre_process.
+  sep_apply store_term_unfold.
+  unfold NULL.
+  entailer!.
+Qed.
+
+Lemma proof_of_separate_imply_which_implies_wit_6 : separate_imply_which_implies_wit_6.
+Proof.
+  pre_process.
+  sep_apply store_term'_Const; unfold NULL in *.
+  Intros ty ct.
+  Exists ty ct.
+  rewrite <- H3.
+  entailer!.
+  lia.
+  lia.
+Qed. 
+
+Lemma proof_of_check_list_gen_entail_wit_2 : check_list_gen_entail_wit_2.
+Proof. Admitted. 
+
+Lemma proof_of_check_list_gen_return_wit_1 : check_list_gen_return_wit_1.
+Proof. Admitted. 
+
+Lemma proof_of_check_list_gen_return_wit_2_1 : check_list_gen_return_wit_2_1.
+Proof. Admitted. 
+
+Lemma proof_of_check_list_gen_return_wit_2_2 : check_list_gen_return_wit_2_2.
+Proof. Admitted. 
+
+Lemma proof_of_check_list_gen_return_wit_3 : check_list_gen_return_wit_3.
+Proof. Admitted. 
+
+Lemma proof_of_check_list_gen_which_implies_wit_1 : check_list_gen_which_implies_wit_1.
+Proof. Admitted. 
+
+Lemma proof_of_check_list_gen_which_implies_wit_2 : check_list_gen_which_implies_wit_2.
+Proof. Admitted. 
+
+Lemma proof_of_check_list_gen_which_implies_wit_3 : check_list_gen_which_implies_wit_3.
+Proof. Admitted. 
+
+Lemma proof_of_thm_apply_return_wit_1_1 : thm_apply_return_wit_1_1.
+Proof.
+  pre_process.
+  unfold store_solve_res.
+  assert ((thm_app t l g) = SRTList (gen_pre tst g)) .
+  2:{
+    rewrite H6.
+    unfold restypeID.
+    Exists retval_2.
+    entailer!.
+    admit.
+  }
+Admitted.
+
+Lemma proof_of_thm_apply_return_wit_1_2 : thm_apply_return_wit_1_2.
+Proof.
+  pre_process.
+Admitted.
+
+Lemma proof_of_thm_apply_return_wit_1_3 : thm_apply_return_wit_1_3.
+Proof.
+  pre_process.
+  entailer!.
+Admitted.
+
+Lemma proof_of_thm_apply_which_implies_wit_1 : thm_apply_which_implies_wit_1.
+Proof.
+  pre_process.
+  Exists 0 0.
+  unfold store_solve_res.
+  unfold restypeID, NULL.
+  entailer!.
+Qed.
+
+Lemma proof_of_thm_apply_which_implies_wit_2 : thm_apply_which_implies_wit_2.
+Proof.
+  pre_process.
+  unfold store_term_res.
+  destruct (thm_subst t l) eqn:E.
+  - Exists t0.
+    entailer!.
+  - entailer!.
+Qed. 
+
+Lemma proof_of_thm_apply_which_implies_wit_3 : thm_apply_which_implies_wit_3.
+Proof.
+  pre_process.
+  rewrite H.
+  Exists 0.
+  entailer!.
+Admitted.
+
